Replaced "x mem list: by "x : (set list)". Replaced "remove" by "removeAll". Removed integer numbers from "firstPos", "preceeds" and "currentLevel".

thys/SATSolverVerification/MoreList.thy
@@ -1,7 +1,6 @@
-(*    Title:              SATSolverVerification/MyList.thy
-      ID:                 $Id: MoreList.thy,v 1.2 2008-07-27 14:23:32 lsf37 Exp $
+(*    Title:              SATSolverVerification/MoreList.thy
+      ID:                 $Id: MoreList.thy,v 1.3 2008-08-06 15:27:21 filipmaric Exp $
       Author:             Filip Maric
-      Maintainer:         Filip Maric <filip at matf.bg.ac.yu>
 *)
 
 header{* MoreList *}
@@ -9,30 +8,13 @@ header{* MoreList *}
 theory MoreList
 imports Main Multiset
 begin
-text{* Theory contains some additional lemmas and functions for the @{term List} datatype. *}
+
+text{* Theory contains some additional lemmas and functions for the
+@{term List} datatype. Warning: some of these notions are obsolete
+because they already exist in {\em List.thy} in similiar form. *}
 
 (*********************************************************)
-(*                      mem                              *)
-(*********************************************************)
-subsection{* @{text mem} - list membership *}
-lemma nonEmptyList: 
-  assumes "x mem list"
-  shows  "list \<noteq> []"
-using assms
-by (induct list) auto
-
-lemma memAppend: 
-"x mem (list1 @ list2) = (x mem list1 \<or> x mem list2)"
-by (induct list1) auto
-
-lemma nonemptyIsHeadTail: 
-  assumes "list \<noteq> []"
-  shows "\<exists> x list'. list = x # list'"
-using assms
-by (induct list) auto
-
-(*********************************************************)
-(*               last \<and> butlast                         *)
+(*               last and butlast                        *)
 (*********************************************************)
 subsection{* @{term "last"} and @{term "butlast"} - last element of list and elements before it *}
 lemma listEqualsButlastAppendLast: 
@@ -41,22 +23,18 @@ lemma listEqualsButlastAppendLast:
 using assms
 by (induct list) auto
 
-lemma lastListMemList [simp]: 
+lemma lastListInList [simp]: 
   assumes "list \<noteq> []"
-  shows "last list mem list"
+  shows "last list \<in> set list"
 using assms
 by (induct list) auto
 
-lemma memButlastImpliesMemList: 
-  assumes "x mem (butlast list)"
-  shows "x mem list"
-using assms
+lemma butlastIsSubset: 
+  shows "set (butlast list) \<subseteq> set list"
 by (induct list) (auto split: split_if_asm)
 
-lemma memListImpliesMemButlastOrLast: 
-  assumes "x mem list" 
-  shows "x mem butlast list \<or> x = last list"
-using assms
+lemma setListIsSetButlastAndLast: 
+  shows "set list \<subseteq> set (butlast list) \<union> {last list}" 
 by (induct list) auto
 
 lemma butlastAppend: 
@@ -64,163 +42,99 @@ lemma butlastAppend:
 by (induct list1) auto
 
 (*********************************************************)
-(*                   remove                              *)
+(*                   removeAll                           *)
 (*********************************************************)
-subsection{* @{term remove} - element removal *}
+subsection{* @{term removeAll} - element removal *}
 
-text{* Function @{term "remove"} removes all occurences of a given element from a list *}
+text{* Function @{term "removeAll"} - removes all occurences of a given element from a list. *}
 
 consts
-remove :: "'a => 'a list => 'a list"
+removeAll :: "'a => 'a list => 'a list"
 primrec
-"remove x [] = []"
-"remove x (h#t) = (if x=h then (remove x t) else h#(remove x t))"
+"removeAll x [] = []"
+"removeAll x (h#t) = (if x=h then (removeAll x t) else h#(removeAll x t))"
 
-lemma removeAppend [simp]: 
-  shows "remove x (l1 @ l2) = remove x l1 @ remove x l2"
+lemma removeAll_set: 
+  shows "set (removeAll a list) = set list - {a}"
+by (induct list) auto
+
+lemma removeAll_id:
+  assumes "a \<notin> set list"
+  shows "removeAll a list = list"
+using assms
+by (induct list) auto
+
+lemma removeAll_append [simp]: 
+  shows "removeAll x (l1 @ l2) = removeAll x l1 @ removeAll x l2"
 by (induct l1) auto
 
-lemma memRemoveImpliesMemList:
-  assumes "x mem remove a l"
-  shows "x mem l"
-using assms
-by (induct l) (auto split: split_if_asm)
-
-lemma memRemoveImpliesNotRemoved:
-  assumes "x mem remove a l"
-  shows "x \<noteq> a"
-using assms
-by (induct l) (auto split: split_if_asm)
-
-lemma removedNotMemRemove: 
-  shows "\<not> x mem (remove x l)"
-by (induct l) auto
-
-lemma memListImpliesMemRemoveOrRemoved:
-  assumes "x mem l" 
-  shows "x mem remove a l \<or> x=a"
-using assms
-by (induct l) auto
-
-lemma memRemoveIffMemListAndNotRemoved: 
-  shows "x mem remove e l = (x mem l \<and> x \<noteq> e)"
-by (induct l) auto
-
-lemma removeNonMember:
-  assumes "\<not> a mem list"
-  shows "remove a list = list"
-using assms
-by (induct list) auto
-
-(* TODO: remove - easy consequence of memRemoveImpliesMemList and memAppend *)
-lemma memRemoveL1AppendL2: 
-  assumes "x mem remove a l1 @ l2"
-  shows "x mem (l1 @ l2)"
-using assms
-by (induct l1) (auto split: split_if_asm)
-
-lemma setRemove: "set list \<subseteq> {a} \<union> set (remove a list)"
-by (induct list) auto
-
-lemma setRemoveSubset:
-  shows "set (remove x a) \<subseteq> set a"
-by (induct a) auto
-
-lemma setRemoveIff:
-  assumes "x mem a"
-  shows "{x} \<union> set (remove x a) = set a" (is "?lhs = ?rhs")
-proof
-  show "?rhs \<subseteq> ?lhs"
-    by (induct a) auto
-next
-  show "?lhs \<subseteq> ?rhs"
-    using assms
-  proof (induct a)
-    case (Cons y a')
-    thus ?case
-    proof (cases "x = y")
-      case True
-      thus ?thesis
-	using setRemoveSubset[of "y" "a'"]
-	by auto
-    next
-      case False
-      with `x mem y # a'` 
-      have "x mem a'"
-	by simp
-      hence "{x} \<union> set (remove x a') \<subseteq> set a'"
-	using Cons(1)
-	by simp
-      thus ?thesis
-	by auto
-    qed
-  qed simp
-qed
-
-lemma multisetRemoveIff:
-  assumes "distinct a" "x mem a"
-  shows "multiset_of a = {#x#} + multiset_of (remove x a)"
+lemma removeAll_multiset:
+  assumes "distinct a" "x \<in> set a"
+  shows "multiset_of a = {#x#} + multiset_of (removeAll x a)"
 using assms
 proof (induct a)
   case (Cons y a')
   thus ?case
   proof (cases "x = y")
     case True
-    with `distinct (y # a')` `x mem y # a'`
-    have "\<not>  x mem a'"
-      by (auto iff: mem_iff)
-    hence "remove x a' = a'"
-      by (rule removeNonMember)
+    with `distinct (y # a')` `x \<in> set (y # a')`
+    have "\<not>  x \<in> set a'"
+      by auto
+    hence "removeAll x a' = a'"
+      by (rule removeAll_id)
     with `x = y` show ?thesis
       by (simp add: union_commute)
   next
     case False
-    with `x mem y # a'` 
-    have "x mem a'"
+    with `x \<in> set (y # a')` 
+    have "x \<in> set a'"
       by simp
     with `distinct (y # a')`
     show ?thesis
       using Cons(1)
-      by (auto iff: mem_iff simp add: union_assoc)
+      by (auto simp add: union_assoc)
   qed
 qed simp
- 
-lemma removeMap:
+
+lemma removeAll_map:
   assumes "\<forall> x y. x \<noteq> y \<longrightarrow> f x \<noteq> f y"
-  shows "remove (f x) (map f a) = map f (remove x a)"
+  shows "removeAll (f x) (map f a) = map f (removeAll x a)"
 using assms
 by (induct a arbitrary: x) auto
 
+ 
 (*********************************************************)
 (*                   uniq                                *)
 (*********************************************************)
-subsection{* @{term uniq} - no duplicate elements *}
-text{* @{term "(uniq list)"} holds iff there are no repeated elements in a list *}
+subsection{* @{term uniq} - no duplicate elements. *}
+text{* @{term "(uniq list)"} holds iff there are no repeated elements
+in a list.  Obsolete: same as @{term "distinct"} in {\em List.thy}. *}
+
 consts
 uniq :: "'a list => bool"
 primrec
 "uniq [] = True"
-"uniq (h#t) = (\<not> h mem t \<and> uniq t)"
+"uniq (h#t) = (h \<notin> set t \<and> uniq t)"
 
 lemma uniqAppend: 
   assumes "uniq (l1 @ l2)" 
   shows "uniq l1" "uniq l2"
 using assms
-by (induct l1) (auto simp add: memAppend)
+by (induct l1) auto
 
 lemma uniqAppendIff: 
   "uniq (l1 @ l2) = (uniq l1 \<and> uniq l2 \<and> set l1 \<inter> set l2 = {})" (is "?lhs = ?rhs")
-by (induct l1) (auto simp add: mem_iff)
+by (induct l1) auto
 
 lemma uniqAppendElement: 
   assumes "uniq l" 
-  shows "\<not> e mem l = uniq (l @ [e])"
+  shows "e \<notin> set l = uniq (l @ [e])"
 using assms
-by (induct l) (auto split: split_if_asm simp add: memAppend)
+by (induct l) (auto split: split_if_asm)
 
 lemma uniqImpliesNotLastMemButlast:
   assumes "uniq l"
-  shows "\<not> last l mem butlast l"
+  shows "last l \<notin> set (butlast l)"
 proof (cases "l = []")
   case True
   thus ?thesis
@@ -231,7 +145,8 @@ next
   hence "l = butlast l @ [last l]"
     by (rule listEqualsButlastAppendLast)
   moreover
-  with `uniq l` have "uniq (butlast l)"
+  with `uniq l` 
+  have "uniq (butlast l)"
     using uniqAppend[of "butlast l" "[last l]"]
     by simp
   ultimately
@@ -243,7 +158,7 @@ qed
 
 lemma uniqButlastNotUniqListImpliesLastMemButlast: 
   assumes "uniq (butlast l)" "\<not> uniq l" 
-  shows "last l mem butlast l"
+  shows "last l \<in> set (butlast l)"
 proof (cases "l = []")
   case True
   thus ?thesis
@@ -261,255 +176,155 @@ qed
 
 lemma uniqRemdups:
   shows "uniq (remdups x)"
-by (induct x) (auto simp add: mem_iff)
-
-(*********************************************************)
-(*                   intLength                           *)
-(*********************************************************)
-subsection{* @{term intLength} - length of a list *}
-
-consts intLength :: "'a list => int"
-primrec 
-"intLength [] = 0"
-"intLength (h#t) = 1 + intLength(t)"
-
-lemma intLengthGeqZero:
-  shows "intLength l >= 0"
-by (induct "l") auto
-
-lemma intLengthNonEmptyGeq1:
-  assumes "list \<noteq> []"
-  shows "intLength list >= 1"
-using assms
-by (induct list) (auto simp add:intLengthGeqZero)
-
-lemma intLengthAppend:
-  shows "intLength (a @ b) = intLength a + intLength b"
-by (induct "a") auto
+by (induct x) auto
 
 (*********************************************************)
 (*                   firstPos                            *)
 (*********************************************************)
-subsection {* @{term firstPos} - index of an element *}
+subsection {* @{term firstPos} - first position of an element *}
+text{* @{term "firstPos"} returns the zero-based index of the first
+  occurence of an element int a list, or the length of the list if the
+  element does not occur. *}
 
-text{* @{term "firstPos"} returns the zero-based index of the first occurence of an element
-  int a list, or -1 if the element does not occur *}
-
-consts firstPos_aux :: "'a => 'a list => int"
+consts firstPos :: "'a => 'a list => nat"
 primrec
-"firstPos_aux a [] = 0"
-"firstPos_aux a (h # t) = (if a = h then 0 else 1 + (firstPos_aux a t))"
-
-definition  firstPos :: "'a => 'a list => int"
-where
-firstPos_def: "firstPos a l == (if a mem l then (firstPos_aux a l) else -1)"
-
-
-lemma firstPos_auxGeqZero: "firstPos_aux a list >= 0"
-by (induct list) auto
+"firstPos a [] = 0"
+"firstPos a (h # t) = (if a = h then 0 else 1 + (firstPos a t))"
 
 lemma firstPosEqualZero:
   shows "(firstPos a (m # M') = 0) = (a = m)"
-proof
-  assume "firstPos a (m # M') = 0"
-  hence "a mem (m # M')" "firstPos_aux a (m # M') = 0"
-    unfolding firstPos_def
-    by (auto split: split_if_asm)
-  {
-    assume "a \<noteq> m"
-    with `firstPos_aux a (m # M') = 0`
-    have "1 + firstPos_aux a M' = 0"
-      by simp
-    hence False
-      using firstPos_auxGeqZero[of "a" "M'"]
-      by simp
-  }
-  thus "a = m"
-    by auto
-next
-  assume "a = m"
-  thus "firstPos a (m # M') = 0"
-    unfolding firstPos_def
-    by auto
-qed
+by (induct M') auto
 
-lemma firstPosGeqZero:
-  assumes "a mem list" 
-  shows "firstPos a list >= 0"
+lemma firstPosLeLength: 
+  assumes "a \<in> set l"
+  shows "firstPos a l < length l"
 using assms
-unfolding firstPos_def
-by (auto simp add:firstPos_auxGeqZero)
-
-lemma firstPosLeqLength: 
-  assumes "a mem l"
-  shows "firstPos a l < intLength l"
-using assms
-unfolding firstPos_def
-proof (induct l)
-  case (Cons m l')
-  thus ?case
-  proof (cases "a = m")
-    case True
-    thus ?thesis
-      using intLengthGeqZero[of "l'"]
-      by simp
-  next
-    case False
-    with `a mem (m # l')`
-    have "a mem l'"
-      by simp
-    with Cons(1)
-    have "firstPos a l' < intLength l'"
-      unfolding firstPos_def
-      by simp
-    thus ?thesis
-      unfolding firstPos_def
-      using False
-      by auto
-  qed
-qed simp
+by (induct l) auto
 
 lemma firstPosAppend: 
-  assumes "a mem l" 
+  assumes "a \<in> set l" 
   shows "firstPos a l = firstPos a (l @ l')"
 using assms
-unfolding firstPos_def
-by (induct l) (auto simp add: memAppend)
+by (induct l) auto
 
 lemma firstPosAppendNonMemberFirstMemberSecond: 
-  assumes "\<not> a mem l1" and  "a mem l2"
-  shows "firstPos a (l1 @ l2) = intLength l1 + firstPos a l2"
+  assumes "a \<notin> set l1" and  "a \<in> set l2"
+  shows "firstPos a (l1 @ l2) = length l1 + firstPos a l2"
 using assms
-proof (induct l1)
-  case (Cons m l1')
-  from `\<not> a mem m # l1'` have "\<not>  a mem l1'" "a \<noteq> m"
-    by (auto split: split_if_asm)
-  with `a mem l2` Cons(1)
-  have "firstPos a (l1' @ l2) = intLength l1' + firstPos a l2"
-    by simp
-  moreover
-  from `a \<noteq> m` `a mem l2` have 
-    "firstPos a ((m # l1') @ l2) = 1 + firstPos a (l1' @ l2)"
-    unfolding firstPos_def
-    by (auto simp add: memAppend)
-  ultimately
-  show ?case
-    by simp
-qed simp
+by (induct l1) auto
 
 lemma firstPosDomainForElements: 
-  shows "(firstPos a l >= 0 \<and> firstPos a l < intLength l) = a mem l" (is "?lhs = ?rhs")
-proof
-  assume "?lhs"
-  thus "?rhs"
-    unfolding firstPos_def
-    by (auto split: split_if_asm)
-next
-  assume "?rhs"
-  thus "?lhs"
-    using firstPosGeqZero[of "a" "l"]
-    using firstPosLeqLength[of "a" "l"]
+  shows "(0 \<le> firstPos a l \<and> firstPos a l < length l) = (a \<in> set l)" (is "?lhs = ?rhs")
+  by (induct l) auto
+
+lemma firstPosEqual: 
+  assumes "a \<in> set l" and "b \<in> set l" 
+  shows "(firstPos a l = firstPos b l) = (a = b)" (is "?lhs = ?rhs")
+proof-
+  {
+    assume "?lhs"
+    hence "?rhs"
+      using assms
+    proof (induct l)
+      case (Cons m l')
+      {
+	assume "a = m"
+	have "b = m"
+	proof-
+	  from `a = m` 
+	  have "firstPos a (m # l') = 0"
+	    by simp
+	  with Cons 
+	  have "firstPos b (m # l') = 0"
+	    by simp
+	  with `b \<in> set (m # l')` 
+	  have "firstPos b (m # l') = 0"
+	    by simp
+	  thus ?thesis
+	    using firstPosEqualZero[of "b" "m" "l'"]
+	    by simp
+	qed
+	with `a = m` 
+	have ?case
+	  by simp
+      }
+      note * = this
+      moreover
+      {
+	assume "b = m"
+	have "a = m"
+	proof-
+	  from `b = m` 
+	  have "firstPos b (m # l') = 0"
+	    by simp
+	  with Cons 
+	  have "firstPos a (m # l') = 0"
+	    by simp
+	  with `a \<in> set (m # l')` 
+	  have "firstPos a (m # l') = 0"
+	    by simp
+	  thus ?thesis
+	    using firstPosEqualZero[of "a" "m" "l'"]
+	    by simp
+	qed
+	with `b = m` 
+	have ?case
+	  by simp
+      }
+      note ** = this
+      moreover
+      {
+	assume Q: "a \<noteq> m" "b \<noteq> m"
+	from Q `a \<in> set (m # l')`
+	have "a \<in> set l'"
+	  by simp
+	from Q `b \<in> set (m # l')`
+	have "b \<in> set l'"
+	  by simp
+	from `a \<in> set l'` `b \<in> set l'` Cons
+	have "firstPos a l' = firstPos b l'"
+	  by (simp split: split_if_asm)
+	with Cons 
+	have ?case
+	  by (simp split: split_if_asm)
+      }
+      note *** = this
+      moreover
+      {
+	have "a = m \<or> b = m \<or> a \<noteq> m \<and> b \<noteq> m"
+	  by auto
+      }
+      ultimately
+      show ?thesis
+      proof (cases "a = m")
+	case True
+	thus ?thesis
+	  by (rule *)
+      next
+	case False
+	thus ?thesis
+	proof (cases "b = m")
+	  case True
+	  thus ?thesis
+	    by (rule **)
+	next
+	  case False
+	  with `a \<noteq> m` show ?thesis
+	    by (rule ***)
+	qed
+      qed
+    qed simp
+  } thus ?thesis
     by auto
 qed
 
-lemma firstPosEqual: 
-  assumes "a mem l" and "b mem l" and "firstPos a l = firstPos b l"
-  shows "a = b"
-using assms
-unfolding firstPos_def
-proof (induct l)
-case (Cons m l')
-hence P: "firstPos_aux a (m # l') = firstPos_aux b (m # l')"
-  by (simp split: split_if_asm)
-{
-  assume "a = m"
-  have "b = m"
-  proof-
-    from `a = m` have "firstPos_aux a (m # l') = 0"
-      by simp
-    with P have "firstPos_aux b (m # l') = 0"
-      by simp
-    with `b mem (m # l')` have
-      "firstPos b (m # l') = 0"
-      unfolding firstPos_def
-      by simp
-    thus ?thesis
-    using firstPosEqualZero[of "b" "m" "l'"]
-    by simp
-  qed
-  with `a = m` have ?case
-    by simp
-}
-note * = this
-moreover
-{
-  assume "b = m"
-  have "a = m"
-  proof-
-    from `b = m` have "firstPos_aux b (m # l') = 0"
-      by simp
-    with P have "firstPos_aux a (m # l') = 0"
-      by simp
-    with `a mem (m # l')` have
-      "firstPos a (m # l') = 0"
-      unfolding firstPos_def
-      by simp
-    thus ?thesis
-    using firstPosEqualZero[of "a" "m" "l'"]
-    by simp
-  qed
-  with `b = m` have ?case
-    by simp
-}
-note ** = this
-moreover
-{
-  assume Q: "a \<noteq> m" "b \<noteq> m"
-  from Q `a mem (m # l')`
-  have "a mem l'"
-    by simp
-  from Q `b mem (m # l')`
-  have "b mem l'"
-    by simp
-  from `a mem l'` `b mem l'` P Q
-  have "firstPos_aux a l' = firstPos_aux b l'"
-    by (simp split: split_if_asm)
-  with Cons Q have ?case
-    by (simp split: split_if_asm)
-}
-note *** = this
-moreover
-{
-  have "a = m \<or> b = m \<or> a \<noteq> m \<and> b \<noteq> m"
-    by auto
-}
-ultimately
-show ?thesis
-proof (cases "a = m")
-  case True
-  thus ?thesis
-    by (rule *)
-next
-  case False
-  thus ?thesis
-  proof (cases "b = m")
-    case True
-    thus ?thesis
-      by (rule **)
-  next
-    case False
-    with `a \<noteq> m` show ?thesis
-      by (rule ***)
-  qed
-qed
-qed simp
 (*********************************************************)
 (*                   preceeds                            *)
 (*********************************************************)
 subsection{* @{term preceeds} - ordering relation induced by @{term firstPos} *}
 definition preceeds :: "'a => 'a => 'a list => bool"
 where
-"preceeds a b l == (a mem l \<and> b mem l \<and>  firstPos a l <= firstPos b l)"
+"preceeds a b l == (a \<in> set l \<and> b \<in> set l \<and>  firstPos a l <= firstPos b l)"
 
 lemma noElementsPreceedsFirstElement: 
   assumes "a \<noteq> b"
@@ -517,16 +332,15 @@ lemma noElementsPreceedsFirstElement:
 proof-
   {
     assume "preceeds a b (b # list)"
-    hence "a mem (b # list)" "firstPos a (b # list) <= 0"
+    hence "a \<in> set (b # list)" "firstPos a (b # list) <= 0"
       unfolding preceeds_def
-      unfolding firstPos_def
       by (auto split: split_if_asm)
     hence  "firstPos a (b # list) = 0"
-      using firstPosGeqZero[of "a" "b # list"]
-      by simp
-    with `a \<noteq> b` have False
+      by auto
+    with `a \<noteq> b` 
+    have False
       using firstPosEqualZero[of "a" "b" "list"]
-      by (simp del: firstPos_def)
+      by simp
   }
   thus ?thesis
     by auto
@@ -536,45 +350,47 @@ lemma preceedsAppend:
   assumes "preceeds a b l" 
   shows "preceeds a b (l @ l')"
 proof-
-  from `preceeds a b l` have "a mem l" "b mem l" "firstPos a l \<le> firstPos b l"
+  from `preceeds a b l` 
+  have "a \<in> set l" "b \<in> set l" "firstPos a l \<le> firstPos b l"
     unfolding preceeds_def
     by (auto split: split_if_asm)
   thus ?thesis
     using firstPosAppend[of "a" "l" "l'"]
     using firstPosAppend[of "b" "l" "l'"]
     unfolding preceeds_def
-    by (simp add:memAppend)
+    by simp
 qed
 
 lemma preceedsMemberHeadMemberTail: 
-  assumes "a mem l1" and "\<not> b mem l1" and "b mem l2"
+  assumes "a \<in> set l1" and "b \<notin> set l1" and "b \<in> set l2"
   shows "preceeds a b (l1 @ l2)"
 proof-
-  from `a mem l1` have "firstPos a l1 < intLength l1"
-    using firstPosLeqLength [of "a" "l1"]
+  from `a \<in> set l1` 
+  have "firstPos a l1 < length l1"
+    using firstPosLeLength [of "a" "l1"]
     by simp
   moreover
-  from `a mem l1` have "firstPos a (l1 @ l2) = firstPos a l1"
+  from `a \<in> set l1` 
+  have "firstPos a (l1 @ l2) = firstPos a l1"
     using firstPosAppend[of "a" "l1" "l2"]
     by simp
   moreover
-  from `\<not> b mem l1` `b mem l2`
-  have "firstPos b (l1 @ l2) = intLength l1 + firstPos b l2"
+  from `b \<notin> set l1` `b \<in> set l2`
+  have "firstPos b (l1 @ l2) = length l1 + firstPos b l2"
     by (rule firstPosAppendNonMemberFirstMemberSecond)
   moreover
-  from `b mem l2` 
-  have "firstPos b l2 >= 0"
-    by (rule firstPosGeqZero)
+  have "firstPos b l2 \<ge> 0"
+    by auto
   ultimately
   show ?thesis
     unfolding preceeds_def
-    using `a mem l1` `b mem l2`
-    by (simp add: memAppend)
+    using `a \<in> set l1` `b \<in> set l2`
+    by simp
 qed
 
 
 lemma preceedsReflexivity: 
-  assumes "a mem l"
+  assumes "a \<in> set l"
   shows "preceeds a a l"
 using assms
 unfolding preceeds_def
@@ -582,7 +398,7 @@ by simp
 
 lemma preceedsTransitivity: 
   assumes 
-  "a mem l" and "b mem l" and "c mem l"
+  "a \<in> set l" and "b \<in> set l" and "c \<in> set l"
   "preceeds a b l" and "preceeds b c l" 
   shows 
   "preceeds a c l"
@@ -592,7 +408,7 @@ by auto
 
 lemma preceedsAntisymmetry: 
   assumes
-  "a mem l" and "b mem l" and
+  "a \<in> set l" and "b \<in> set l" and
   "preceeds a b l" and "preceeds b a l"
   shows
   "a = b"
@@ -608,7 +424,7 @@ proof-
 qed
 
 lemma preceedsTotalOrder: 
-  assumes "a mem l" and "b mem l"
+  assumes "a \<in> set l" and "b \<in> set l"
   shows "a=b \<or> preceeds a b l \<or> preceeds b a l"
 using assms
 unfolding preceeds_def
@@ -624,22 +440,23 @@ proof (induct list)
       assume "a = l"
       have ?case
       proof-
-	from `a = l` have "firstPos (f a) (map f (l # list')) = 0"
+	from `a = l` 
+	have "firstPos (f a) (map f (l # list')) = 0"
 	  using firstPosEqualZero[of "f a" "f l" "map f list'"]
 	  by simp
 	moreover
 	from `preceeds a b (l # list')` 
-	have "b mem l # list'"
+	have "b \<in> set (l # list')"
 	  unfolding preceeds_def
 	  by simp
-	hence "f b mem map f (l # list')"
-	  by (auto simp add: mem_iff)
-	hence "firstPos (f b) (map f (l # list')) >= 0"
-	  using firstPosGeqZero[of "f b" "map f (l # list')"]
-	  by simp
+	hence "f b \<in> set (map f (l # list'))"
+	  by auto
+	moreover
+	hence "firstPos (f b) (map f (l # list')) \<ge>  0"
+	  by auto
 	ultimately
 	show ?thesis
-	  using `a = l` `f b mem map f (l # list')`
+	  using `a = l` `f b \<in> set (map f (l # list'))`
 	  unfolding preceeds_def
 	  by simp
       qed
@@ -663,11 +480,11 @@ proof (induct list)
       have "f a \<noteq> f l" "f b \<noteq> f l"
 	by auto
       from `preceeds a b (l # list')` 
-      have "b mem l # list'" "a mem l # list'" "firstPos a (l # list') <= firstPos b (l # list')"
+      have "b \<in> set(l # list')" "a \<in> set(l # list')" "firstPos a (l # list') \<le> firstPos b (l # list')"
 	unfolding preceeds_def
 	by auto
-      with `a \<noteq> l` `b \<noteq> l` have "a mem list'" "b mem list'" "firstPos a list' <= firstPos b list'"
-	unfolding firstPos_def
+      with `a \<noteq> l` `b \<noteq> l` 
+      have "a \<in> set list'" "b \<in> set list'" "firstPos a list' \<le> firstPos b list'"
 	by auto
       hence "preceeds a b list'"
 	unfolding preceeds_def
@@ -678,7 +495,6 @@ proof (induct list)
       with `f a \<noteq> f l` `f b \<noteq> f l`
       have ?case
 	unfolding preceeds_def
-	unfolding firstPos_def
 	by auto
     }
     ultimately 
@@ -700,25 +516,27 @@ proof(induct list)
   show ?case
   proof-
     from `preceeds a b (l # list')` 
-    have "a mem l # list'" "b mem l # list'" "firstPos a (l # list') <= firstPos b (l # list')"
+    have "a \<in> set(l # list')" "b \<in> set(l # list')" "firstPos a (l # list') \<le> firstPos b (l # list')"
       unfolding preceeds_def
       by auto
-    from `f a` `a mem l # list'` have "a mem filter f (l # list')"
-      by (auto simp add: mem_iff)
+    from `f a` `a \<in> set(l # list')` 
+    have "a \<in> set(filter f (l # list'))"
+      by auto
     moreover
-    from `f b` `b mem (l # list')` have "b mem filter f (l # list')"
-      by (auto simp add: mem_iff)
+    from `f b` `b \<in> set(l # list')` 
+    have "b \<in> set(filter f (l # list'))"
+      by auto
     moreover
-    have "firstPos a (filter f (l # list')) <= firstPos b (filter f (l # list'))"
+    have "firstPos a (filter f (l # list')) \<le> firstPos b (filter f (l # list'))"
     proof- 
       {
 	assume "a = l"
-	with `f a` have "firstPos a (filter f (l # list')) = 0"
-	  unfolding firstPos_def
+	with `f a` 
+	have "firstPos a (filter f (l # list')) = 0"
 	  by auto
-	with `b mem (filter f (l # list'))` have ?thesis
-	  using firstPosGeqZero[of "b" "(filter f (l # list'))"]
-	  by simp
+	with `b \<in> set (filter f (l # list'))` 
+	have ?thesis
+	  by auto
       }
       moreover
       {
@@ -733,15 +551,17 @@ proof(induct list)
       moreover
       {
 	assume "a \<noteq> l" "b \<noteq> l"
-	with `preceeds a b (l # list')` have "firstPos a list' <= firstPos b list'"
+	with `preceeds a b (l # list')` 
+	have "firstPos a list' \<le> firstPos b list'"
 	  unfolding preceeds_def
-	  unfolding firstPos_def
 	  by auto
 	moreover
-	from `a \<noteq> l` `a mem l # list'` have "a mem list'"
+	from `a \<noteq> l` `a \<in> set (l # list')` 
+	have "a \<in> set list'"
 	  by simp
 	moreover
-	from `b \<noteq> l` `b mem l # list'` have "b mem list'"
+	from `b \<noteq> l` `b \<in> set (l # list')` 
+	have "b \<in> set list'"
 	  by simp
 	ultimately
 	have "preceeds a b list'"
@@ -753,7 +573,6 @@ proof(induct list)
 	with `a \<noteq> l` `b \<noteq> l`
 	have ?thesis
 	  unfolding preceeds_def
-	  unfolding firstPos_def
 	  by auto
       }
       ultimately
@@ -789,14 +608,15 @@ proof-
 	  {
 	    fix a'
 	    assume "(a', ?aMin) \<in> preceedsOrder list"
-	    hence "a mem list"
+	    hence "a \<in> set list"
 	      unfolding preceedsOrder_def
 	      unfolding preceeds_def
 	      by simp
 	    with `a \<in> Q`
-	    have "a mem ?listQ"
+	    have "a \<in> set ?listQ"
 	      by (induct list) auto
-	    with `?listQ = []` have "False"
+	    with `?listQ = []` 
+	    have "False"
 	      by simp
 	    hence "a' \<notin> Q"
 	      by simp
@@ -811,14 +631,15 @@ proof-
       next
 	case False
 	let ?aMin = "hd ?listQ"
-	from False have "?aMin \<in> Q"
+	from False 
+	have "?aMin \<in> Q"
 	  by (induct list) auto
 	have "\<forall> a'. (a', ?aMin) \<in> preceedsOrder list \<longrightarrow> a' \<notin> Q"
 	proof
 	  fix a'
 	  {
 	    assume "(a', ?aMin) \<in> preceedsOrder list"
-	    hence "a' mem list" "preceeds a' ?aMin list" "a' \<noteq> ?aMin"
+	    hence "a' \<in> set list" "preceeds a' ?aMin list" "a' \<noteq> ?aMin"
 	      unfolding preceedsOrder_def
 	      unfolding preceeds_def
 	      by auto
@@ -830,7 +651,8 @@ proof-
 		have "preceeds a' ?aMin ?listQ"
 		    using preceedsFilter[of "a'" "?aMin" "list" "\<lambda> x. x \<in> Q"]
 		    by blast
-		from `a' \<noteq> ?aMin` have "\<not> preceeds a' (hd ?listQ) (hd ?listQ # tl ?listQ)"
+		from `a' \<noteq> ?aMin` 
+		have "\<not> preceeds a' (hd ?listQ) (hd ?listQ # tl ?listQ)"
 		  by (rule noElementsPreceedsFirstElement)
 		with False `preceeds a' ?aMin ?listQ`
 		have "False"
@@ -856,21 +678,14 @@ qed
 (*********************************************************)
 (*                   prefix                              *)
 (*********************************************************)
-subsection{* @{term prefix} - prefixes of list *}
-
-text{* Check if a list is a prefix of another list *}
+subsection{* @{term isPrefix} - prefixes of list. *}
+text{* Check if a list is a prefix of another list. Obsolete: similiar
+notion is defined in {\em List\_prefixes.thy}. *}
 
 consts
 isPrefix :: "'a list => 'a list => bool"
 defs
 isPrefix_def: "isPrefix p t == \<exists> s. p @ s = t"
-
-lemma memPrefixImpliesMemList:
-  assumes "isPrefix p l" and "x mem p" 
-  shows "x mem l"
-using assms
-unfolding isPrefix_def
-by (auto simp add: memAppend)
 
 lemma prefixIsSubset:
   assumes "isPrefix p l"
@@ -894,14 +709,14 @@ proof-
 qed
 
 lemma firstPosPrefixElement: 
-  assumes "isPrefix p l" and "a mem p"
+  assumes "isPrefix p l" and "a \<in> set p"
   shows "firstPos a p = firstPos a l"
 proof-
   from `isPrefix p l` obtain s
     where "p @ s = l"
     unfolding isPrefix_def
     by auto
-  with `a mem p` 
+  with `a \<in> set p` 
   show ?thesis
     using firstPosAppend[of "a" "p" "s"]
     by simp
@@ -909,7 +724,7 @@ qed
 
 lemma laterInPrefixRetainsPreceeds: 
   assumes 
-  "isPrefix p l" and "preceeds a b l" and "b mem p"
+  "isPrefix p l" and "preceeds a b l" and "b \<in> set p"
   shows 
   "preceeds a b p"
 proof-
@@ -917,42 +732,42 @@ proof-
     where "p @ s = l"
     unfolding isPrefix_def
     by auto
-  from `preceeds a b l` have "a mem l" "b mem l" "firstPos a l \<le> firstPos b l"
+  from `preceeds a b l` 
+  have "a \<in> set l" "b \<in> set l" "firstPos a l \<le> firstPos b l"
     unfolding preceeds_def
     by (auto split: split_if_asm)
 
-  from `p @ s = l` `b mem p` have "firstPos b l = firstPos b p"
+  from `p @ s = l` `b \<in> set p` 
+  have "firstPos b l = firstPos b p"
     using firstPosAppend [of "b" "p" "s"]
     by simp
 
   show ?thesis
-  proof (cases "a mem p")
+  proof (cases "a \<in> set p")
     case True
-    from `p @ s = l` `a mem p` have "firstPos a l = firstPos a p"
+    from `p @ s = l` `a \<in> set p` 
+    have "firstPos a l = firstPos a p"
       using firstPosAppend [of "a" "p" "s"]
       by simp
 
     from `firstPos a l = firstPos a p` `firstPos b l = firstPos b p` `firstPos a l \<le> firstPos b l`
-    `a mem p` `b mem p`
+    `a \<in> set p` `b \<in> set p`
     show ?thesis
       unfolding preceeds_def
       by simp
   next
     case False
-    from `\<not> a mem p` `a mem l` `p @ s = l`
-    have "a mem s"
-      by (auto simp add: memAppend)
-    with `\<not> a mem p` `p @ s = l`
-    have "firstPos a l = intLength p + firstPos a s"
+    from `a \<notin> set p` `a \<in> set l` `p @ s = l`
+    have "a \<in> set s"
+      by auto
+    with `a \<notin> set p` `p @ s = l`
+    have "firstPos a l = length p + firstPos a s"
       using firstPosAppendNonMemberFirstMemberSecond[of "a" "p" "s"]
       by simp
     moreover
-    from `a mem s` have "firstPos a s >= 0"
-      by (rule firstPosGeqZero)
-    moreover
-    from `b mem p` 
-    have "firstPos b p < intLength p"
-      by (rule firstPosLeqLength)
+    from `b \<in> set p` 
+    have "firstPos b p < length p"
+      by (rule firstPosLeLength)
     ultimately
     show ?thesis
       using `firstPos b l = firstPos b p` `firstPos a l \<le> firstPos b l`
@@ -960,24 +775,23 @@ proof-
   qed
 qed
 
-
 (*********************************************************)
 (*                       List diff                       *)
 (*********************************************************)
-subsection{* @{term "list_diff"} - difference of lists *}
+subsection{* @{term "list_diff"} - the set difference operation on two lists. *}
 
 consts 
 list_diff :: "'a list \<Rightarrow> 'a list \<Rightarrow> 'a list"
 primrec 
 "list_diff x [] = x"
-"list_diff x (y#ys) = list_diff (remove y x) ys"
+"list_diff x (y#ys) = list_diff (removeAll y x) ys"
 
 lemma [simp]: 
   shows "list_diff [] y = []"
 by (induct y) auto
 
 lemma [simp]: 
-  shows "list_diff (x # xs) y = (if x mem y then list_diff xs y else x # list_diff xs y)"
+  shows "list_diff (x # xs) y = (if x \<in> set y then list_diff xs y else x # list_diff xs y)"
 proof (induct y arbitrary: xs)
   case (Cons y ys)
   thus ?case
@@ -988,7 +802,7 @@ proof (induct y arbitrary: xs)
   next
     case False
     thus ?thesis
-    proof (cases "x mem ys")
+    proof (cases "x \<in> set ys")
       case True
       thus ?thesis
 	using Cons
@@ -1003,43 +817,43 @@ proof (induct y arbitrary: xs)
 qed simp
 
 lemma listDiffIff:
-  shows "(x mem a \<and> \<not> x mem b) = x mem list_diff a b"
+  shows "(x \<in> set a \<and> x \<notin> set b) = (x \<in> set (list_diff a b))"
 by (induct a) auto
 
-lemma listDiffDoubleRemove: 
-  assumes "x mem a"
+lemma listDiffDoubleRemoveAll: 
+  assumes "x \<in> set a"
   shows "list_diff b a = list_diff b (x # a)"
 using assms
 by (induct b) auto
 
-lemma removeListDiff[simp]:
-  shows "remove x (list_diff a b) = list_diff (remove x a) b"
+lemma removeAllListDiff[simp]:
+  shows "removeAll x (list_diff a b) = list_diff (removeAll x a) b"
 by (induct a) auto
 
-lemma listDiffRemoveNonMember:
-  assumes "\<not> x mem a"
-  shows "list_diff a b = list_diff a (remove x b)"
+lemma listDiffRemoveAllNonMember:
+  assumes "x \<notin> set a"
+  shows "list_diff a b = list_diff a (removeAll x b)"
 using assms
 proof (induct b arbitrary: a)
   case (Cons y b')
-  from `\<not> x mem a` have "\<not> x mem remove y a"
-    using setRemoveSubset[of "y" "a"]
-    by (auto iff: mem_iff)
+  from `x \<notin> set a` 
+  have "x \<notin> set (removeAll y a)"
+    by (auto simp add: removeAll_set)
   thus ?case
   proof (cases "x = y")
     case False
     thus ?thesis
       using Cons(2)
-      using Cons(1)[of "remove y a"]
-      using `\<not> x mem (remove y a)`
+      using Cons(1)[of "removeAll y a"]
+      using `x \<notin> set (removeAll y a)`
       by auto
   next
     case True
     thus ?thesis
-      using Cons(1)[of "remove y a"]
-      using `\<not> x mem a`
-      using `\<not> x mem remove y a`
-      by (auto simp add: removeNonMember)
+      using Cons(1)[of "removeAll y a"]
+      using `x \<notin> set a`
+      using `x \<notin> set (removeAll y a)`
+      by (auto simp add: removeAll_id)
   qed
 qed simp
 
@@ -1047,77 +861,23 @@ lemma listDiffMap:
   assumes "\<forall> x y. x \<noteq> y \<longrightarrow> f x \<noteq> f y"
   shows "map f (list_diff a b) = list_diff (map f a) (map f b)"
 using assms
-by (induct b arbitrary: a) (auto simp add: removeMap)
+by (induct b arbitrary: a) (auto simp add: removeAll_map)
 
 (*********************************************************)
 (*                       Remdups                         *)
 (*********************************************************)
 subsection{* @{term remdups} - removing duplicates *}
-lemma remdupsRemoveCommute[simp]:
-  shows "remdups (remove a list) = remove a (remdups list)"
-proof (induct list)
-  case (Cons l list')
-  thus ?case
-  proof (cases "a = l")
-    case True
-    with Cons show ?thesis
-      by auto
-  next
-    case False
-    with Cons
-    show ?thesis
-    proof-
-      {
-	assume "l \<in> set list'"
-	with `a \<noteq> l`
-	have "l \<in> set (remove a list')"
-	  using setRemove[of "list'" "a"]
-	  by auto
-      }
-      moreover
-      {
-	assume "l \<notin> set list'"
-	with `a \<noteq> l`
-	have "l \<notin> set (remove a list')"
-	  using memRemoveImpliesMemList[of "l" "a" "list'"]
-	  by (auto simp add: mem_iff)
-      }
-      ultimately 
-      show ?thesis
-	using Cons
-	by auto
-    qed
-  qed
-qed simp
+lemma remdupsRemoveAllCommute[simp]:
+  shows "remdups (removeAll a list) = removeAll a (remdups list)"
+by (induct list) (auto simp add: removeAll_set)
 
 lemma remdupsAppend: 
   shows "remdups (a @ b) = remdups (list_diff a b) @ remdups b"
 proof (induct a)
   case (Cons x a')
   thus ?case
-  proof (cases "x mem b")
-    case True
-    thus ?thesis
-      using Cons
-      by (simp add: mem_iff)
-  next
-    case False
-    thus ?thesis
-    proof (cases "x mem a'")
-      case True
-      from `x mem a'` `\<not> x mem b` 
-      show ?thesis
-	using Cons
-	using listDiffIff[of "x" "a'" "b"]
-	by (auto iff: mem_iff)
-    next
-      case False
-      thus ?thesis
-	using Cons
-	using listDiffIff[of "x" "a'" "b"]
-	by (auto iff: mem_iff)
-    qed
-  qed
+    using listDiffIff[of "x" "a'" "b"]
+    by auto
 qed simp
 
 lemma remdupsAppendSet: 
@@ -1129,53 +889,52 @@ proof (induct a)
 next
   case (Cons x a')
   thus ?case
-  proof (cases "x mem a'")
+  proof (cases "x \<in> set a'")
     case True
     thus ?thesis
       using Cons
-      using listDiffDoubleRemove[of "x" "a'" "b"]
-      by (simp add: mem_iff)
+      using listDiffDoubleRemoveAll[of "x" "a'" "b"]
+      by simp
   next
     case False
     thus ?thesis
-    proof (cases "x mem b")
+    proof (cases "x \<in> set b")
       case True
       show ?thesis
       proof-
 	have "set (remdups (x # a') @ remdups (list_diff b (x # a'))) = 
 	  set (x # remdups a' @ remdups (list_diff b (x # a')))"
-	  using `\<not> x mem a'`
+	  using `x \<notin> set a'`
 	  by auto
-	also have "\<dots> = set (x # remdups a' @ remdups (list_diff (remove x b) a'))"
+	also have "\<dots> = set (x # remdups a' @ remdups (list_diff (removeAll x b) a'))"
 	  by auto
-	also have "\<dots> = set (x # remdups a' @ remdups (remove x (list_diff b a')))"
+	also have "\<dots> = set (x # remdups a' @ remdups (removeAll x (list_diff b a')))"
 	  by simp
-	also have "\<dots> = set (remdups a' @ x # remdups (remove x (list_diff b a')))"
+	also have "\<dots> = set (remdups a' @ x # remdups (removeAll x (list_diff b a')))"
 	  by simp
-	also have "\<dots> = set (remdups a' @ x # remove x (remdups (list_diff b a')))"
-	  by (simp only: remdupsRemoveCommute)
-	also have "\<dots> = set (remdups a') \<union> set (x # remove x (remdups (list_diff b a')))"
+	also have "\<dots> = set (remdups a' @ x # removeAll x (remdups (list_diff b a')))"
+	  by (simp only: remdupsRemoveAllCommute)
+	also have "\<dots> = set (remdups a') \<union> set (x # removeAll x (remdups (list_diff b a')))"
 	  by simp
-	also have "\<dots> = set (remdups a') \<union> {x} \<union> set (remove x (remdups (list_diff b a')))"
+	also have "\<dots> = set (remdups a') \<union> {x} \<union> set (removeAll x (remdups (list_diff b a')))"
 	  by simp
 	also have "\<dots> = set (remdups a') \<union> set (remdups (list_diff b a'))"
 	proof-
-	  from `\<not> x mem a'` `x mem b`
-	  have "x mem list_diff b a'"
+	  from `x \<notin> set a'` `x \<in> set b`
+	  have "x \<in> set (list_diff b a')"
 	    using listDiffIff[of "x" "b" "a'"]
 	    by simp
-	  hence "x mem remdups (list_diff b a')"
-	    by (auto iff: mem_iff)
-	  thus ?thesis
-	    using setRemoveIff[of "x" "remdups (list_diff b a')"]
+	  hence "x \<in> set (remdups (list_diff b a'))"
 	    by auto
+	  thus ?thesis
+	    by (auto simp add: removeAll_set)
 	qed
 	also have "\<dots> = set (remdups (a' @ b))"
 	  using Cons(1)
 	  by simp
 	also have "\<dots> = set (remdups ((x # a') @ b))"
-	  using `x mem b`
-	  by (simp add: mem_iff)
+	  using `x \<in> set b`
+	  by simp
 	finally show ?thesis
 	  by simp
       qed
@@ -1185,14 +944,13 @@ next
       proof-
 	have "set (remdups (x # a') @ remdups (list_diff b (x # a'))) = 
 	  set (x # (remdups a') @ remdups (list_diff b (x # a')))"
-	  using `\<not> x mem a'`
+	  using `x \<notin> set a'`
 	  by auto
-	also have "\<dots> = set (x # remdups a' @ remdups (list_diff (remove x b) a'))"
+	also have "\<dots> = set (x # remdups a' @ remdups (list_diff (removeAll x b) a'))"
 	  by auto
 	also have "\<dots> = set (x # remdups a' @ remdups (list_diff b a'))"
-	  using `\<not> x mem b`
-	  using removeNonMember[of "x" "b"]
-	  by simp
+	  using `x \<notin> set b`
+	  by (auto simp add: removeAll_id)
 	also have "\<dots> = {x} \<union> set (remdups (a' @ b))"
 	  using Cons(1)
 	  by simp
@@ -1214,16 +972,16 @@ proof (induct a)
 next
   case (Cons x a')
   thus ?case
-  proof (cases "x mem a'")
+  proof (cases "x \<in> set a'")
     case True
     thus ?thesis
       using Cons
-      using listDiffDoubleRemove[of "x" "a'" "b"]
-      by (simp add: mem_iff)
+      using listDiffDoubleRemoveAll[of "x" "a'" "b"]
+      by simp
     next
     case False
     thus ?thesis
-    proof (cases "x mem b")
+    proof (cases "x \<in> set b")
       case True
       show ?thesis
       proof-
@@ -1231,41 +989,41 @@ next
 	  multiset_of (x # remdups a' @ remdups (list_diff b (x # a')))"
 	proof-
 	  have "remdups (x # a') = x # remdups a'"
-	    using `\<not> x mem a'`
-	    by (auto iff: mem_iff)
+	    using `x \<notin> set a'`
+	    by auto
 	  thus ?thesis
 	    by simp
 	qed
-	also have "\<dots> = multiset_of (x # remdups a' @ remdups (list_diff (remove x b) a'))"
+	also have "\<dots> = multiset_of (x # remdups a' @ remdups (list_diff (removeAll x b) a'))"
 	  by auto
-	also have "\<dots> = multiset_of (x # remdups a' @ remdups (remove x (list_diff b a')))"
+	also have "\<dots> = multiset_of (x # remdups a' @ remdups (removeAll x (list_diff b a')))"
 	  by simp
-	also have "\<dots> = multiset_of (remdups a' @ x # remdups (remove x (list_diff b a')))"
+	also have "\<dots> = multiset_of (remdups a' @ x # remdups (removeAll x (list_diff b a')))"
 	  by (simp add: union_assoc)
-	also have "\<dots> = multiset_of (remdups a' @ x # remove x (remdups (list_diff b a')))"
-	  by (simp only: remdupsRemoveCommute)
-	also have "\<dots> = multiset_of (remdups a') + multiset_of (x # remove x (remdups (list_diff b a')))"
+	also have "\<dots> = multiset_of (remdups a' @ x # removeAll x (remdups (list_diff b a')))"
+	  by (simp only: remdupsRemoveAllCommute)
+	also have "\<dots> = multiset_of (remdups a') + multiset_of (x # removeAll x (remdups (list_diff b a')))"
 	  by simp
-	also have "\<dots> = multiset_of (remdups a') + {#x#} + multiset_of (remove x (remdups (list_diff b a')))"
+	also have "\<dots> = multiset_of (remdups a') + {#x#} + multiset_of (removeAll x (remdups (list_diff b a')))"
 	  by (simp add: union_assoc) (simp add: union_commute)
 	also have "\<dots> = multiset_of (remdups a') + multiset_of (remdups (list_diff b a'))"
 	proof-
-	  from `\<not> x mem a'` `x mem b`
-	  have "x mem (list_diff b a')"
+	  from `x \<notin> set a'` `x \<in> set b`
+	  have "x \<in> set (list_diff b a')"
 	    using listDiffIff[of "x" "b" "a'"]
 	    by simp
-	  hence "x mem (remdups (list_diff b a'))"
-	    by (auto iff: mem_iff)
+	  hence "x \<in> set (remdups (list_diff b a'))"
+	    by auto
 	  thus ?thesis
-	    using multisetRemoveIff[of "remdups (list_diff b a')" "x"]
+	    using removeAll_multiset[of "remdups (list_diff b a')" "x"]
 	    by (simp add: union_assoc)
 	qed
 	also have "\<dots> = multiset_of (remdups (a' @ b))"
 	  using Cons(1)
 	  by simp
 	also have "\<dots> = multiset_of (remdups ((x # a') @ b))"
-	  using `x mem b`
-	  by (simp add: mem_iff)
+	  using `x \<in> set b`
+	  by simp
 	finally show ?thesis
 	  by simp
       qed
@@ -1277,23 +1035,23 @@ next
 	  multiset_of (x # remdups a' @ remdups (list_diff b (x # a')))"
 	proof-
 	  have "remdups (x # a') = x # remdups a'"
-	    using `\<not> x mem a'`
-	    by (auto iff: mem_iff)
+	    using `x \<notin> set a'`
+	    by auto
 	  thus ?thesis
 	    by simp
 	qed
-	also have "\<dots> = multiset_of (x # remdups a' @ remdups (list_diff (remove x b) a'))"
+	also have "\<dots> = multiset_of (x # remdups a' @ remdups (list_diff (removeAll x b) a'))"
 	  by auto
 	also have "\<dots> = multiset_of (x # remdups a' @ remdups (list_diff b a'))"
-	  using `\<not> x mem b`
-	  using removeNonMember[of "x" "b"]
+	  using `x \<notin> set b`
+	  using removeAll_id[of "x" "b"]
 	  by simp
 	also have "\<dots> = {#x#} + multiset_of (remdups (a' @ b))"
 	  using Cons(1)
 	  by (simp add: union_commute)
 	also have "\<dots> = multiset_of (remdups ((x # a') @ b))"
-	  using `\<not> x mem a'` `\<not> x mem b`
-	  by (auto iff: mem_iff simp add: union_commute)
+	  using `x \<notin> set a'` `x \<notin> set b`
+	  by (auto simp add: union_commute)
 	finally show ?thesis
 	  by simp
       qed
@@ -1306,6 +1064,10 @@ qed
 (*                       Levi                            *)
 (*********************************************************)
 subsection{* Levi's lemma *}
+
+text{* Obsolete: these two lemmas are already proved as @{term
+append_eq_append_conv2} and @{term append_eq_Cons_conv}. *}
+
 lemma FullLevi: 
   shows "(x @ y = z @ w) = 
                 (x = z \<and> y = w \<or> 
